code/ed25519/Hacl.Ed25519.fst
@@ -1,5 +1,7 @@
 module Hacl.Ed25519
 
+
+
 let sign signature secret msg len =
   Hacl.Impl.Ed25519.Sign.sign signature secret msg len
 
@@ -8,3 +10,40 @@ let verify public msg len signature =
 
 let secret_to_public out secret =
   Hacl.Impl.Ed25519.SecretToPublic.secret_to_public out secret
+
+let secret_to_public_expanded out secret_expanded =
+  Hacl.Impl.Ed25519.SecretToPublic.secret_to_public_expanded out secret_expanded
+
+let point_add_compressed o p1 p2 = 
+  push_frame();
+  let buf1 = create (Hacl.Cast.uint64_to_sint64 0uL) 20ul in
+  let buf2 = create (Hacl.Cast.uint64_to_sint64 0uL) 20ul in
+  let buf3 = create (Hacl.Cast.uint64_to_sint64 0uL) 20ul in
+  let res1 = Hacl.Impl.Ed25519.PointDecompress.point_decompress buf1 p1 in
+  let res2 = Hacl.Impl.Ed25519.PointDecompress.point_decompress buf2 p2 in
+  let res = 
+    if (res1 && res2) then (
+      Hacl.Impl.Ed25519.PointAdd.point_add buf3 buf1 buf2;
+      Hacl.Impl.Ed25519.PointCompress.point_compress o buf3;
+      true
+      )
+    else false in
+  pop_frame(); 
+  res
+
+let point_mul_compressed o scalar p = 
+  push_frame();
+  let buf1 = create (Hacl.Cast.uint64_to_sint64 0uL) 20ul in
+  let buf2 = create (Hacl.Cast.uint64_to_sint64 0uL) 20ul in
+  let res1 = Hacl.Impl.Ed25519.PointDecompress.point_decompress buf1 p in
+  let res = if (res1) then (
+      Hacl.Impl.Ed25519.Ladder.point_mul buf2 scalar buf1;
+      Hacl.Impl.Ed25519.PointCompress.point_compress o buf2;
+      true)
+      else false in
+  pop_frame();
+  res
+
+
+let sign_expanded signature secret msg len = 
+  Hacl.Impl.Ed25519.Sign.sign_expanded signature secret msg len
